test: add examples

Grw/Morphism.lean
@@ -1,99 +1,113 @@
 import Aesop
+import Grw.Eauto
 
-def Relation (α : Sort u) := α → α → Prop
+namespace Morphism
 
-def Impl (α β : Prop) : Prop := α → β
+initialize
+  Lean.registerTraceClass `Meta.Tactic.grewrite
 
-def All (α : Type) (P : α -> Prop) := ∀ x : α, P x
+abbrev relation (α : Sort u) := α → α → Prop
 
-def Relation.inverse {α : Sort u} (r : Relation α) : α → α → Prop :=
+def impl (α β : Prop) : Prop := α → β
+
+def all (α : Sort u) (p : α -> Prop) :=
+  ∀x, p x
+
+def relation.inverse {α : Sort u} (r : relation α) : α → α → Prop :=
 λ x y => r y x
 
-postfix:max "⁻¹" => Relation.inverse
+postfix:max "⁻¹" => relation.inverse
 
-class Reflexive {α : Sort u} (rel : Relation α) where
+class Reflexive {α : Sort u} (rel : relation α) where
   rfl : ∀ x, rel x x
 
-class Symmetric {α : Sort u} (rel : Relation α) where
+class Symmetric {α : Sort u} (rel : relation α) where
   symm : ∀ x y, rel x y → rel⁻¹ x y
 
-class Transitive {α : Sort u} (rel : Relation α) where
+class Transitive {α : Sort u} (rel : relation α) where
   trans : ∀ x y z, rel x y → rel y z → rel x z
 
-class Eqiv {r : Relation α} where
-  rel : Reflexive r
-  symm : Symmetric r
-  trans : Transitive r
+class Equiv {α : Sort u} (r : relation α) extends Reflexive r, Symmetric r, Transitive r
 
-instance flipReflexive {α : Sort u} {r : Relation α} [Reflexive r] : Reflexive r⁻¹ :=
+@[aesop unsafe 100% apply]
+instance flipReflexive {α : Sort u} {r : relation α} [Reflexive r] : Reflexive r⁻¹ :=
   Reflexive.mk fun x => by
-    rw [Relation.inverse]
+    rw [relation.inverse]
     apply Reflexive.rfl x
 
-instance implReflexive : Reflexive Impl :=
+@[aesop unsafe 100% apply]
+instance implReflexive : Reflexive impl :=
   Reflexive.mk fun _ => id
 
-instance implTransitive : Transitive Impl :=
+@[aesop unsafe 100% apply]
+instance implTransitive : Transitive impl :=
   Transitive.mk fun _ _ _ pqr pq => pq ∘ pqr
 
-class Subrel {α : Sort u} (q r : Relation α) : Prop where
+class Subrel {α : Sort u} (q r : relation α) : Prop where
   subrelation : ∀ x y, q x y → r x y
 
-instance subrelationRefl {α : Sort u} {r : Relation α} : Subrel r r :=
+@[aesop unsafe 100% apply]
+instance subrelationRefl {α : Sort u} {r : relation α} : Subrel r r :=
   Subrel.mk fun _ _ => id
 
-instance iffImplSubrelation : Subrel Iff Impl :=
+@[aesop unsafe 100% apply]
+instance iffImplSubrelation : Subrel Iff impl :=
   Subrel.mk fun _ _ pq hq => propext pq ▸ hq
 
-instance iffInverseImplSubrelation : Subrel Iff Impl⁻¹ :=
+@[aesop unsafe 100% apply]
+instance iffInverseImplSubrelation : Subrel Iff impl⁻¹ :=
   Subrel.mk fun _ _ pq hq => propext pq ▸ hq
 
-class Proper {α : Sort u} (r : Relation α) (m : α) where
+class Proper {α : Sort u} (r : relation α) (m : α) where
   proper : r m m
 
-instance reflexiveProper {α : Sort u} {r : Relation α} [Reflexive r] (x : α) : Proper r x :=
+@[aesop unsafe 100% apply]
+instance reflexiveProper {α : Sort u} {r : relation α} [Reflexive r] (x : α) : Proper r x :=
   Proper.mk <| Reflexive.rfl x
 
-def respectful {α β : Sort u} (r : Relation α) (r' : Relation β) : Relation (α → β) :=
+def respectful {α : Sort u} {β : Sort v} (r : relation α) (r' : relation β) : relation (α → β) :=
   fun f g => ∀ x y, r x y → r' (f x) (g y)
 
+@[aesop unsafe 100% apply]
 theorem contrapositive {a b : Prop} :
   (a → b) → ¬ b → ¬ a :=
   fun hab hnb ha => hnb (hab ha)
 
+@[aesop unsafe 100% apply]
 instance notIffMorphism : Proper (respectful Iff Iff) Not :=
   Proper.mk fun _ _ x => Iff.intro (contrapositive x.mpr) (contrapositive x.mp)
 
 notation:55 r " ⟹ " r' => respectful r r'
 notation:55 r " ⟶ " r' => respectful r⁻¹ r'
 
-instance contraposedMorphism : Proper (Impl ⟶ Impl) Not := by
+@[aesop unsafe 100% apply]
+instance contraposedMorphism : Proper (impl ⟶ impl) Not := by
   apply Proper.mk
   intro a b f na
-  rw [Relation.inverse, Not] at *
+  rw [relation.inverse, Not] at *
   apply contrapositive (f) (na)
 
-instance transMorphism [Transitive r] : Proper (r ⟶ r ⟹ Impl) r := by
+@[aesop unsafe 100% apply]
+instance transMorphism [Transitive r] : Proper (r ⟶ r ⟹ impl) r := by
   apply Proper.mk
   intro a b iab c d r r'
-  rw [Relation.inverse] at iab
+  rw [relation.inverse] at iab
   apply Transitive.trans
   apply iab
   apply Transitive.trans <;>
   assumption
 
-def pointwiseRelation (α : Sort u) {β : Sort u} (r : Relation β) : Relation (α → β) :=
+def pointwiseRelation (α : Sort u) {β : Sort u} (r : relation β) : relation (α → β) :=
   fun f g => ∀ a, r (f a) (g a)
 
-def all (α : Type) (p : α -> Prop) :=
-  ∀x, p x
-
+@[aesop unsafe 100% apply]
 instance flipProper [mor : Proper (rα ⟹ rβ ⟹ rφ) f] : Proper (rβ ⟹ rα ⟹ rφ) (flip f) := by
   apply Proper.mk
   intro b₁ b₂ rb a₁ a₂ ra
   apply mor.proper
   repeat assumption
 
+@[aesop unsafe 100% apply]
 instance respectfulSubrelation [rs : Subrel r₂ r₁] [ss : Subrel s₁ s₂] : Subrel (r₁ ⟹ s₁) (r₂ ⟹ s₂) := by
   apply Subrel.mk
   intro f f' p x y rxy
@@ -101,6 +115,7 @@ instance respectfulSubrelation [rs : Subrel r₂ r₁] [ss : Subrel s₁ s₂] :
   apply p
   exact rs.subrelation x y rxy
 
+@[aesop unsafe 100% apply]
 instance : Proper (Subrel ⟹ Subrel) (@pointwiseRelation α β) := by
   apply Proper.mk
   intro rb rb' sr
@@ -109,59 +124,28 @@ instance : Proper (Subrel ⟹ Subrel) (@pointwiseRelation α β) := by
   apply sr.subrelation
   apply hfg
 
+@[aesop unsafe 100% apply]
 instance subrelationPointwise α [sub : @Subrel β r r'] : Subrel (pointwiseRelation α r) (pointwiseRelation α r') := by
   apply Subrel.mk
   intro f g pr a
   apply sub.subrelation
   apply pr
 
-inductive Tlist : Type (u+1)
-| tnil : Tlist
-| tcons : Type u → Tlist → Tlist
+def relationEquivalence : relation (relation α) :=
+  Eq
 
-local infixr:66 " ∷ " => Tlist.tcons
---infixr:67 " :: " => List.cons
-
-def arrows : Tlist → Type u → Type u
-| Tlist.tnil, r => r
-| Tlist.tcons A l', r => A → arrows l' r
-
-def predicate (l : Tlist) := arrows l Prop
-
-def binaryRelation (α : Type) := predicate (α ∷ α ∷ Tlist.tnil)
-
-def pointwiseLifting (op : binaryRelation Prop) (l : Tlist) : binaryRelation (predicate l) :=
-  match l with
-  | .tnil => fun r r' => op r r'
-  | _ ∷ tl => fun r r' => ∀ x, pointwiseLifting op tl (r x) (r' x)
-
-def predicateEquivalence {l : Tlist} : binaryRelation (predicate l) :=
-  pointwiseLifting Iff l
-
-def relationEquivalence {α : Type} : Relation (Relation α) :=
-    @predicateEquivalence (_ ∷ _ ∷ Tlist.tnil)
-
-instance proper α : Proper (@relationEquivalence α ⟹ Eq ⟹ Iff) Proper := by
+@[aesop unsafe 100% apply]
+instance proper (α : Sort u) : Proper (relationEquivalence ⟹ Eq ⟹ Iff) (@Proper α) := by
   apply Proper.mk
   intro r r' hreq a b heq
   apply Iff.intro
   . intro hprp
-    rw [relationEquivalence] at hreq
-    rw [predicateEquivalence] at hreq
-    rw [← heq]
     apply Proper.mk
-    replace hreq := hreq a a
-    rw [pointwiseLifting] at hreq
-    rw [← hreq]
+    rw [← heq, ← hreq]
     apply hprp.proper
   . intro hprp
-    rw [relationEquivalence] at hreq
-    rw [predicateEquivalence] at hreq
     apply Proper.mk
-    replace hreq := hreq a a
-    rw [pointwiseLifting] at hreq
-    rw [hreq]
-    rw [heq]
+    rw [hreq, heq]
     apply hprp.proper
 
 /-only apply at the top of the goal with the subrelation flag set to true
@@ -171,11 +155,16 @@ theorem subrelationProper [p : Proper r₁ m] [sr : Subrel r₁ r₂] : Proper r
   apply p.proper)
 -/
 
+-- TODO: instance «partial» [@Proper (α → β) (r ⟹ r') m] [@Proper α r x] : Proper r' (m x) := sorry
+
+@[aesop unsafe 100% apply]
 instance properInverse [p : Proper r m] : Proper r⁻¹ m := Proper.mk p.proper
 
-theorem inverseInvol α (r : Relation α) : r⁻¹⁻¹ = r := rfl
+@[aesop unsafe 100% apply]
+theorem inverseInvol α (r : relation α) : r⁻¹⁻¹ = r := rfl
 
-theorem inverseArrow α (ra : Relation α) β (rb : Relation β) : (ra ⟹ rb)⁻¹ = ra⁻¹ ⟹ rb⁻¹ := by
+@[aesop unsafe 100% apply]
+theorem inverseArrow α (ra : relation α) β (rb : relation β) : (ra ⟹ rb)⁻¹ = ra⁻¹ ⟹ rb⁻¹ := by
   funext f g
   apply propext
   apply Iff.intro <;>
@@ -183,11 +172,13 @@ theorem inverseArrow α (ra : Relation α) β (rb : Relation β) : (ra ⟹ rb)�
     apply h
     exact hra
 
-class Normalizes {α} (m m' : Relation α) where
+class Normalizes {α} (m m' : relation α) where
   normalizes : m = m'⁻¹
 
+@[aesop unsafe 100% apply]
 theorem norm1 α r : @Normalizes α r (r⁻¹) := Normalizes.mk rfl
 
+@[aesop unsafe 100% apply]
 theorem norm2 [n₁ : @Normalizes β r₀ r₁] [n₂ : @Normalizes β u₀ u₁] : Normalizes (r₀ ⟹ u₀) (r₁ ⟹ u₁) := Normalizes.mk (by
   funext f g
   apply propext
@@ -196,3 +187,122 @@ theorem norm2 [n₁ : @Normalizes β r₀ r₁] [n₂ : @Normalizes β u₀ u₁
     intro h x y hr
     apply h
     exact hr)
+
+/- Instances Sébastien Michelland added
+
+instance: Equiv (@Eq α) where
+  rfl  := Eq.refl
+  symm  := by
+    intros
+    apply Eq.symm
+    assumption
+  trans := by
+    intros
+    apply Eq.trans
+    repeat assumption
+
+instance: Equiv Iff where
+  rfl  := Iff.refl
+  symm  := by
+    intros
+    apply Iff.symm
+    assumption
+  trans := by
+    intros
+    apply Iff.trans
+    repeat assumption
+
+instance {R : relation α} [PER R] : Proper (R ⟹ R ⟹ Iff) R := by
+  apply Proper.mk
+  intro a b rab c d rcd
+  apply Iff.intro
+  intros
+  apply Transitive.trans
+  apply Symmetric.symm
+  assumption
+  intros
+  apply Transitive.trans
+  repeat assumption
+  intros
+  apply Transitive.trans
+  apply Transitive.trans
+  repeat assumption
+  apply Symmetric.symm
+  assumption
+
+instance {R : relation α} [PER R] : Proper (R ⟹ Eq ⟹ Iff) R := by
+  apply Proper.mk
+  intro a b rab c d hcd
+  apply Iff.intro
+  intro rac
+  apply Transitive.trans
+  apply Symmetric.symm
+  assumption
+  rw [hcd] at rac
+  assumption
+  intro rbd
+  apply Transitive.trans
+  assumption
+  rw [← hcd] at rbd
+  assumption
+
+instance {R : relation α} [PER R] : Proper (Eq ⟹ R ⟹ Iff) R := by
+  apply Proper.mk
+  intro a b hab c d rcd
+  apply Iff.intro
+  intro rac
+  apply Transitive.trans
+  rw [← hab]
+  repeat assumption
+  intro rbd
+  rw [hab]
+  apply Transitive.trans
+  assumption
+  apply Symmetric.symm
+  assumption
+
+instance Proper_flip [P: Proper (Rα ⟹ Rβ ⟹ Rγ) f]:
+    Proper (Rβ ⟹ Rα ⟹ Rγ) (flip f) where
+  proper _ _ h_b _ _ h_a := P.proper _ _ h_a _ _ h_b
+
+instance Subrel_Eq [Reflexive R]: Subrel Eq R where
+  subrelation h := by
+    intro y heq
+    simp_all
+    apply Reflexive.rfl
+
+instance respectfulPER [hr₁ : PER r₁] [hr₂ : PER r₂]: PER (r₁ ⟹ r₂) where
+  symm h g hg x y h₁ := by
+    apply hr₂.symm
+    apply hg
+    apply Symmetric.symm
+    assumption
+  trans f g h fg gh a b rab := by
+    apply hr₂.trans
+    apply fg
+    exact rab
+    apply gh
+    apply Transitive.trans
+    apply Symmetric.symm
+    repeat assumption
+
+instance properAndIff: Proper (Iff ⟹ Iff ⟹ Iff) And :=
+  ⟨fun _ _ hx _ _ hy => by simp [hx, hy]⟩
+
+instance properOrIff: Proper (Iff ⟹ Iff ⟹ Iff) Or :=
+  ⟨fun _ _ hx _ _ hy => by simp [hx, hy]⟩
+
+instance properNotIff: Proper (Iff ⟹ Iff) Not :=
+  ⟨fun _ _ h => by simp [h]⟩
+
+theorem reflexiveSubrel (r : relation α): Subrel r r := by
+  apply Subrel.mk
+  intros
+  assumption
+
+end Morphism
+
+-/
+eauto_create_db grewrite
+--eauto_hint Morphism.reflexiveSubrel : grewrite
+eauto_hint Morphism.Reflexive.rfl : grewrite
