Grw.lean
@@ -2,3 +2,6 @@
 -- Import modules here that should be built as part of the library.
 import Grw.Morphism
 import Grw.Tactic
+import Grw.Test
+import Grw.Eauto
+import Grw.EautoHints
