Grw/Eauto.lean
@@ -1,0 +1,316 @@
+/-
+# Basic typeclass inference with backtracking
+
+This file implements a very rough imitation of Coq's `eauto`. It is used to
+close a set of goals (here: typeclass queries) that may share metavariables,
+with backtracking and hints with priorities. Unlike the standard synthesis
+algorithm, this will instantiate metavariables.
+
+General idea to solve a goal:
+
+1. Try to apply hypotheses from the local context; the "cost" is the number of
+   parameters (subgoals, roughly). If one unifies, solve subgoals recursively.
+   Depending on whether we solve normally (`eauto`) or as a custom typeclass
+   algorithm (`typeclasses_eauto`), typeclass parameters are either synthesized
+   immediately or left as subgoals.
+
+2. Try to apply hints from provided databases. These can be:
+   - Constant hints, ie. theorems. The method is the same as for hypotheses.
+   - Extern hints (a pattern + a tactic + a fixed cost).
+
+3. When solving as a custom typeclass algorithm, try instances given by
+   `SynthInstance.getInstances` (ie. instances that unify with the goal).
+
+4. Recursively solve all the subgoals *and* the entire pending stack (which is
+   affected by current decisions due to metavariables being unified). If that
+   fails, backtrack to the next applicable hint.
+
+5. If not hint applies or a pre-determined maximum depth is reached, fail.
+
+Future wishlist:
+- Caching. There is *a ton* of redundant work during backtracking.
+  This requires being smart with metavariables, since the same "goal" can be
+  traversed with different metavariables assignments.
+- A rough idea of when/why this algorithm will fail to find solutions that
+  `Lean.Meta.SynthInstance` finds.
+- Solve the most egregious performance issues.
+
+Realistic TODO list:
+- TODO: Sort hypotheses, constant hints and typeclass instances by priority
+  based on `getExpectedNumArgs`.
+- TODO: Figure out how to apply extern hints
+-/
+
+import Grw.EautoHints
+
+open Lean Meta Elab Tactic
+
+/-
+## apply_no_synth
+
+This variant of `apply` does not try to solve implicit instances by typeclass
+resolution, and instead adds them as subgoals. It also ignores dependent
+subgoals and case naming (for the purpose of `eauto`).
+-/
+
+namespace ApplyNoSynth
+
+private def throwApplyError {α} (mvarId : MVarId) (eType : Expr) (targetType : Expr) : MetaM α :=
+  throwTacticEx `apply mvarId m!"failed to unify{indentExpr eType}\nwith{indentExpr targetType}"
+
+private def dependsOnOthers (mvar : Expr) (otherMVars : Array Expr) : MetaM Bool :=
+  otherMVars.anyM fun otherMVar => do
+    if mvar == otherMVar then
+      return false
+    else
+      let otherMVarType ← inferType otherMVar
+      return (otherMVarType.findMVar? fun mvarId => mvarId == mvar.mvarId!).isSome
+
+private def getNonDependentMVars (mvars : Array Expr) : MetaM (Array MVarId) := do
+  let mut nonDeps := #[]
+  for mvar in mvars do
+    if !(← dependsOnOthers mvar mvars) then
+      nonDeps := nonDeps.push mvar.mvarId!
+  return nonDeps
+
+def _root_.Lean.MVarId.applyNoSynth (mvarId : MVarId) (e : Expr) : MetaM (List MVarId) :=
+  mvarId.withContext do
+    mvarId.checkNotAssigned `apply
+    let targetType ← mvarId.getType
+    let eType      ← inferType e
+    let mut (numArgs, hasMVarHead) ← getExpectedNumArgsAux eType
+    unless hasMVarHead do
+      let targetTypeNumArgs ← getExpectedNumArgs targetType
+      numArgs := numArgs - targetTypeNumArgs
+    let (newMVars, _, eType) ← forallMetaTelescopeReducing eType (some numArgs)
+    unless (← isDefEq eType targetType) do throwApplyError mvarId eType targetType
+    let e ← instantiateMVars e
+    mvarId.assign (mkAppN e newMVars)
+    let newMVars ← newMVars.filterM fun mvar => not <$> mvar.mvarId!.isAssigned
+    let otherMVarIds ← getMVarsNoDelayed e
+    let newMVarIds := (← getNonDependentMVars newMVars) |>.toList
+    let otherMVarIds := otherMVarIds.filter fun mvarId => !newMVarIds.contains mvarId
+    let result := newMVarIds ++ otherMVarIds.toList
+    result.forM (·.headBetaType)
+    return result
+
+end ApplyNoSynth
+
+/-
+## eauto hint commands
+-/
+
+namespace Eauto
+
+elab "#print_eauto_db": command => do
+  let env ← getEnv
+  let e := eautoDatabaseExtension.getState env
+  if e.dbs.size == 0 then
+    logInfo "no hint databases"
+  else
+    logInfo (MessageData.joinSep (e.dbs.toList.map fun db =>
+        m!"in database {db.name}:\n  " ++ toMessageData db)
+      (.ofFormat "\n\n"))
+
+elab "eauto_create_db" dbname:ident: command => do
+  let env ← getEnv
+  let e := eautoDatabaseExtension.getState env
+
+  if e.hasHintDB dbname.getId then
+    throwError "eauto database {dbname} already exists"
+  else
+    setEnv (eautoDatabaseExtension.addEntry env <| .CreateDB dbname.getId)
+
+elab "eauto_hint " cst:ident ":" dbname:ident: command => do
+  let env ← getEnv
+  let e := eautoDatabaseExtension.getState env
+  let hint: Hint ←
+    match env.find? cst.getId with
+    | some _ => pure <| Hint.Constant cst.getId
+    | none => throwError "no such constant {cst}"
+
+  if ! e.hasHintDB dbname.getId then
+    throwError "no eauto database {dbname}"
+  setEnv (eautoDatabaseExtension.addEntry env <| .CreateHint dbname.getId hint)
+
+end Eauto
+
+/-
+## `eauto` and `typeclasses_eauto`
+-/
+
+namespace Eauto
+
+initialize
+  registerTraceClass `Meta.Tactic.eauto
+  registerTraceClass `Meta.Tactic.eauto.goals
+  registerTraceClass `Meta.Tactic.eauto.hints
+  registerTraceClass `Meta.Tactic.eauto.instances
+
+initialize
+  eautoFailedExceptionId : InternalExceptionId ← registerInternalExceptionId `eautoFailed
+
+structure Context where
+  hintDatabases: Array HintDB
+  useTypeclasses: Bool
+  maximumDepth: Nat
+
+abbrev EautoM := ReaderT Context MetaM
+
+def ppSubgoals (subgoals: List MVarId): EautoM MessageData :=
+  let ppOne (m: MVarId) := do
+    -- return toMessageData m -- to print hypotheses
+    return m!"{← ppExpr (← m.getType)}"
+  return MessageData.joinSep (← subgoals.mapM ppOne) (.ofFormat ", ")
+
+instance : MonadBacktrack Meta.SavedState EautoM where
+  saveState := Meta.saveState
+  restoreState s := s.restore
+
+private def throwEautoFailedEx {α: Type _}: EautoM α :=
+  throw <| Exception.internal eautoFailedExceptionId
+
+private def apply' (goal: MVarId) (expr: Expr) (synthInstances: Bool): EautoM (List MVarId) := do
+  if (← goal.isAssigned) then
+    throwEautoFailedEx
+  let goalType ← goal.getType
+  let exprType ← inferType expr
+  let mut (numArgs, hasMVarHead) ← getExpectedNumArgsAux exprType
+  unless hasMVarHead do
+    let targetTypeNumArgs ← getExpectedNumArgs goalType
+    numArgs := numArgs - targetTypeNumArgs
+  let (_, _, exprType) ← forallMetaTelescopeReducing exprType (some numArgs)
+  unless (← isDefEq exprType goalType) do
+    throwEautoFailedEx
+
+  if synthInstances then
+    goal.apply expr
+  else
+    goal.applyNoSynth expr
+
+mutual
+-- Solve the provided goal and continue on with the entire stack.
+partial def solve (goalMVar: MVarId) (depth: Nat) (goalStack: List (Nat × MVarId)): EautoM Unit := do
+  let ctx ← read
+
+  -- Intro any new binders
+  let (new_fvars, goalMVar) ← goalMVar.intros
+  let goalType ← goalMVar.getType
+
+  goalMVar.withContext do
+    if new_fvars.size > 0 then
+      -- TODO: pp.inaccessibleNames doesn't show the names with tombstones?
+      withOptions (pp.sanitizeNames.set . false) do
+        trace[Meta.Tactic.eauto] "intros {new_fvars.size} binders: {goalMVar}"
+
+    -- Try hypotheses
+    for ldecl in ← getLCtx do
+      if ! ldecl.isAuxDecl then
+        if ← tryProgress depth goalStack do
+          let t ← inferType ldecl.toExpr
+          let subgoals ← apply' goalMVar ldecl.toExpr !ctx.useTypeclasses
+          trace[Meta.Tactic.eauto.hints] "applying hypothesis: {ldecl.userName}: {← ppExpr t}"
+          return subgoals
+        then return ()
+
+    -- Try database hints
+    for db in ctx.hintDatabases do
+      for hint in db.hints do
+        if ← tryProgress depth goalStack do
+          match hint with
+          | .Constant name =>
+              let expr ← mkConstWithFreshMVarLevels name
+              let type ← inferType expr
+              let subgoals ← apply' goalMVar expr !ctx.useTypeclasses
+              trace[Meta.Tactic.eauto.hints] "[{db.name}] applying hint: {hint}: {type}"
+              return subgoals
+          | .Extern _ _ _ =>
+              -- TODO: Apply extern hints
+              throwEautoFailedEx
+        then return ()
+
+    -- Try typeclass instances
+    if ctx.useTypeclasses && (← isClass? goalType).isSome then
+      let instances ← SynthInstance.getInstances goalType
+      -- TODO: Use a better measure that eliminates arguments that appear in
+      -- the type of following arguments. And possibly give a lower cost to
+      -- instances whose goals have more constants/less variables.
+      let instances ← instances.mapM (fun e => do return (e.val, ← getExpectedNumArgs (← inferType e.val)))
+      let instances := instances.qsort (fun (_, c₁) (_, c₂) => c₁ < c₂)
+      trace[Meta.Tactic.eauto.instances] "instances: {instances}"
+      for (inst, cost) in instances do
+        if ← tryProgress depth goalStack do
+          let subgoals ← apply' goalMVar inst !ctx.useTypeclasses
+          trace[Meta.Tactic.eauto.hints] "applying instance({cost}): {inst}: {← ppExpr (← inferType inst)}"
+          return subgoals
+        then return ()
+
+    if (← getExprMVarAssignment? goalMVar).isNone then
+      trace[Meta.Tactic.eauto] "failed to close the goal"
+      throwEautoFailedEx
+
+-- Pop a goal off the stack and solve it (along with the rest of the stack, by
+-- backtracking).
+partial def nextGoal: List (Nat × MVarId) → EautoM Unit
+  | [] => pure ()
+  | (depth, goal) :: stack => do
+      if ← goal.isAssigned then
+        nextGoal stack
+      else
+        let ctx ← read
+        let goal_type ← instantiateMVars (← goal.getType)
+        withTraceNode `Meta.Tactic.eauto
+          (fun _ => return m!"goal[{depth}]: {goal_type}") do
+
+          if depth > ctx.maximumDepth then
+            trace[Meta.Tactic.eauto] "maximum depth exceeded"
+            throwEautoFailedEx
+          solve goal depth stack
+
+-- Try to progress with `tac` and finish the stack. Returns whether successful.
+partial def tryProgress (depth: Nat) (stack: List (Nat × MVarId)) (tac: EautoM (List MVarId)): EautoM Bool :=
+  catchInternalId eautoFailedExceptionId
+    (commitIfNoEx do
+      let subgoals ← tac
+      if subgoals != [] then
+        trace[Meta.Tactic.eauto.hints] "subgoals: {← ppSubgoals subgoals}"
+      nextGoal (subgoals.map (depth+1, ·) ++ stack)
+      return true)
+    (fun _ => return false)
+end
+
+def eautoCore (initialGoals: List MVarId): EautoM Unit :=
+  nextGoal (initialGoals.map (0, ·))
+
+def eautoMain (goals: List MVarId) (dbNames: Array Name) (useTypeclasses: Bool): TacticM Bool := do
+  let env ← getEnv
+  let db := eautoDatabaseExtension.getState env
+
+  let eautoCtx: Context := {
+    hintDatabases := ← dbNames.mapM (EautoDB.getDB db ·)
+    useTypeclasses := useTypeclasses
+    maximumDepth := 5
+  }
+
+  catchInternalId eautoFailedExceptionId
+    (Eauto.eautoCore goals |>.run eautoCtx)
+    (fun _ => pure ())
+
+  let success ← goals.allM (fun m => do return (← getExprMVarAssignment? m).isSome)
+  if !success then
+    trace[Meta.Tactic.eauto] "no proof found"
+  return success
+
+end Eauto
+
+elab "eauto" : tactic => do
+  let _ ← Eauto.eautoMain [← getMainGoal] #[] false
+
+elab "typeclasses_eauto" : tactic => do
+  let _ ← Eauto.eautoMain [← getMainGoal] #[] true
+
+elab "eauto" "with" dbs:ident+ : tactic => do
+  let _ ← Eauto.eautoMain [← getMainGoal] (dbs.map TSyntax.getId) false
+
+elab "typeclasses_eauto" "with" dbs:ident+ : tactic => do
+  let _ ← Eauto.eautoMain [← getMainGoal] (dbs.map TSyntax.getId) true
