Grw/EautoHints.lean
@@ -1,0 +1,84 @@
+/-
+## Hint databases and hint declaration
+
+This module handles the registration, import and export of eauto hints.
+-/
+
+import Lean
+open Lean Meta
+
+namespace Eauto
+
+inductive Hint where
+  | Constant (n: Name)
+  | Extern (term: Term) (tactic: TSyntax `tactic) (cost: Nat)
+
+instance : ToMessageData Hint where
+  toMessageData
+    | .Constant n => n
+    | .Extern term tactic cost => m!"Extern {cost}: {term} => {tactic}"
+
+/-
+A top-level command run by modules to create databases, add hints, etc. We keep
+them inside .olean files using a persistent extensions so that hints are
+retained between imports.
+-/
+inductive HintCommand where
+  | CreateDB (name: Name)
+  | CreateHint (databaseName: Name) (hint: Hint)
+
+structure HintDB where
+  name: Name
+  hints: Array Hint
+
+instance: ToMessageData HintDB where
+  toMessageData db :=
+    MessageData.joinSep (db.hints.toList.map toMessageData) (.ofFormat "\n  ")
+
+-- We remember which commands are imported and which ones are original so we
+-- are able to export only the originals
+structure EautoDB where
+  dbs: Array HintDB := #[]
+  moduleCommands: Array HintCommand := #[]
+deriving Inhabited
+
+def EautoDB.findHintDB? (e: EautoDB) (name: Name): Option Nat :=
+  e.dbs.findIdx? (fun db => db.name = name)
+
+def EautoDB.hasHintDB (e: EautoDB) (name: Name): Bool :=
+  e.findHintDB? name |>.isSome
+
+-- We cannot throw errors at this level, so we let the top-level commands
+-- handle it instead and do no-ops here.
+def EautoDB.runCommand (e: EautoDB): HintCommand → EautoDB
+  | .CreateDB name =>
+      if e.hasHintDB name then e
+      else { e with dbs := e.dbs.push { name := name, hints := #[] }}
+  | .CreateHint dbName hint =>
+      match e.findHintDB? dbName with
+      | none => e
+      | some i => { e with
+          dbs := e.dbs.modify i (fun db => { db with hints := db.hints.push hint })}
+
+def EautoDB.addCommand (e: EautoDB) (c: HintCommand): EautoDB :=
+  let e' := e.runCommand c
+  { e' with moduleCommands := e'.moduleCommands.push c }
+
+def EautoDB.importCommands (comms: Array (Array HintCommand)): ImportM EautoDB :=
+  return comms.foldl (fun dbs ac => ac.foldl EautoDB.runCommand dbs) {}
+
+def EautoDB.exportCommands (e: EautoDB): Array HintCommand :=
+  e.moduleCommands
+
+def EautoDB.getDB (e: EautoDB) (name: Name): CoreM HintDB :=
+  match e.dbs.find? (fun db => db.name = name) with
+  | some db => return db
+  | none => throwError m!"no eauto database called {name}"
+
+initialize eautoDatabaseExtension: PersistentEnvExtension HintCommand HintCommand EautoDB ←
+  registerPersistentEnvExtension {
+    mkInitial := return {},
+    addImportedFn := EautoDB.importCommands,
+    addEntryFn := EautoDB.addCommand,
+    exportEntriesFn := EautoDB.exportCommands,
+  }
