Grw/Tactic.lean
@@ -7,8 +7,6 @@
 
 ## Algorithm
 
-
-
 ## Tips from Jannis:
 synth instance finds type class instances
 forall telescopes to move BVars to FVars
@@ -19,16 +17,20 @@ stay in MetaM for core functionality, TacticM entrypoint
 
 import Lean.Elab.Tactic
 import Grw.Morphism
+import Grw.Eauto
+import Grw.EautoHints
 import Batteries
+import Aesop
 
 open Lean
 open Lean.Meta
+open Morphism
 open Lean.Elab.Tactic
 
-def isRelation (e : Expr) : MetaM <| Expr × Expr × Expr := do
-  match e with
-  | .app (.app r a) b => pure (r, a, b)
-  | _ => throwError "Not a relation"
+set_option trace.aesop true
+set_option trace.aesop.ruleSet true
+
+namespace Tactic
 
 /--
 Note from paper:
@@ -37,38 +39,68 @@ given lemma ρ is denoted unify_ρ(Γ, Ψ, τ ). It takes as input a typing envi
 a constraint set and a term and tries to unify the left-hand side of the lemma’s
 applied relation with the term. It uses the same unification algorithm as the one
 used when applying a lemma during a proof.
+
+get lhs of ρ (match for app)
+change all vars in Phi to mvars (forallMetaTelescope)
+isdefeq auf term t
+check which of the newly generated mvars are assigned
+(isAssignedOrDelayedAssigned)
+(<- instanciateMvar $ Expr.mvar ?x1 == Expr.mvar ?x1)
+the ones not assigned -> constraint set
+
+side note:
+unification in t can contain more mvars which could get assigned:
+  + if a rule fails
+  + look up (commitIfSuccess)
 -/
-def unify (Ψ : List MVarId) (t : Expr) (p : Expr) : MetaM <| List MVarId × Expr × Expr × Bool := do
-  let (_, lhs, _) ← isRelation p
-  let unifyable ← isDefEq lhs <| t -- Extends the local context
-  /-
-  TODO:
-    - How to obtain updated constraints?
-    - How to obtain `u` with unification from `t` to `u`?
-    - How to obtain the updated lemma `p`
-  -/
-  pure (Ψ, p, t, unifyable)
+def unify (Ψ : List MVarId) (t : Expr) (p : Expr) : MetaM <| List MVarId × Expr × Expr × Expr × Bool := do
+  match p with
+  | .app (.app r lhs) rhs =>
+    let unifyable ← isDefEq lhs t -- Extends the local context
+    pure (Ψ, r, p, rhs, unifyable)
+  | .forallE _ _ (.app (.app r lhs) rhs) _ =>
+    let (exprs, _, e) ← forallMetaTelescope lhs
+    let unifyable ← isDefEq e t -- Extends the local context
+    let mut Ψ := Ψ
+    for expr in exprs do
+      -- Precondition e is forall
+      -- Invariant expr is a mvar
+      let mvarId := expr.mvarId!
+      let reassigned ← mvarId.isAssignedOrDelayedAssigned
+      if !reassigned then
+        Ψ := Ψ.insert mvarId
+    pure (Ψ, r, p, rhs, unifyable)
+  | _ => throwError "{p} is not a relation"
 
 /--
 Note from paper:
 The variant unify∗ ρ(Γ, Ψ, τ ) tries unification on all subterms and succeeds if at least one
 unification does. The function unify(Γ, Ψ, t, u) does a standard unification of t and u.
 -/
-def unifyStar (Ψ : List MVarId) (t : Expr) (p : Expr) : MetaM <| List MVarId × Expr × Expr × Bool := do
-  let (_, lhs, _) ← isRelation p
-  let b ← IO.mkRef false
-  forEachExpr t fun e => do
-    b.set <| (← isDefEq lhs e) || (← b.get)
-  /-
-  TODO:
-    - How to obtain updated constraints?
-    - How to obtain `u` with unification from `t` to `u`?
-    - How to obtain the updated lemma `p`
-  -/
-  pure (Ψ, p, t, ← b.get)
+def unifyStar (Ψ : List MVarId) (t : Expr) (p : Expr) : MetaM <| List MVarId × Expr × Expr × Expr × Bool := match p with
+  | .app (.app r lhs) rhs => do
+    let b ← IO.mkRef false
+    forEachExpr t fun t' => do
+      b.set <| (← isDefEq lhs t') || (← b.get)
+    pure (Ψ, r, p, rhs, ← b.get)
+  | .forallE _ _ (.app (.app r lhs) rhs) _ => do
+    let (exprs, _, t) ← forallMetaTelescope lhs
+    let b ← IO.mkRef false
+    forEachExpr t fun t' => do
+      b.set <| (← isDefEq lhs t') || (← b.get)
+    let mut Ψ := Ψ
+    for expr in exprs do
+      -- Precondition e is forall
+      -- Invariant expr is a mvar
+      let mvarId := expr.mvarId!
+      let reassigned ← mvarId.isAssignedOrDelayedAssigned
+      if !reassigned then
+        Ψ := Ψ.insert mvarId
+    pure (Ψ, r, p, rhs, ← b.get)
+  | _ => throwError "{t} is not a relation"
 
 def mkRel (T : Expr) :=
-  mkApp (mkConst ``Relation) T
+  mkApp (mkConst ``relation [0]) T
 
 def atom (Ψ : List MVarId) (t : Expr) (p : Expr) : MetaM <| List MVarId × Expr × Expr × Expr := do
   /-
@@ -78,7 +110,7 @@ def atom (Ψ : List MVarId) (t : Expr) (p : Expr) : MetaM <| List MVarId × Expr
   -/
   let T ← inferType t
   let rel ← mkFreshExprMVar <| mkRel T
-  let prp ← mkFreshExprMVar <| mkApp3 (mkConst ``Proper) T rel t
+  let prp ← mkFreshExprMVar <| mkApp3 (mkConst ``Proper [0]) T rel t
   return (Ψ ∪ [rel.mvarId!, prp.mvarId!], rel, t, p)
 
 /--
@@ -87,21 +119,21 @@ def atom (Ψ : List MVarId) (t : Expr) (p : Expr) : MetaM <| List MVarId × Expr
 This output tuple represents the proof sekelton that is used in the proof search.
 -/
 partial def rew (Ψ : List MVarId) (t : Expr) (p : Expr) : MetaM (List MVarId × Expr × Expr × Expr) := do
+  withTraceNode `Meta.Tactic.grewrite (fun _ => return m!"rew Ψ ({t}) ρ") do
   /-
   invariants:
     - p is of type Relation
   -/
-  let (Ψ', p', _u, unifyable) ← unify Ψ t p
+  let (Ψ', r, p', u, unifyable) ← unify Ψ t p
   if unifyable then
-    logInfo "Unify⇓"
-    let (R, _a, _b) ← isRelation p
-    return (Ψ', R, t, p')
-  logInfo "Unify⇑"
+    trace[Meta.Tactic.grewrite] "UNIFY⇓ {t} ↝ {u}"
+    return (Ψ', r, t, p')
+  trace[Meta.Tactic.grewrite] "Unify⇑ {t}"
   match t with
   | .app f e => do
-    logInfo m!"App {t}"
-    let (Ψ, E, f, p) ← rew Ψ f p
-    let (Ψ, F, e, p) ← rew Ψ e p
+    trace[Meta.Tactic.grewrite] "APPSUB ({f}) ({e})"
+    let (Ψ, E, f', pf) ← rew Ψ f p
+    let (Ψ, F, e', pe) ← rew Ψ e p
     /-
     preconditions:
       - t is an application f e
@@ -109,16 +141,18 @@ partial def rew (Ψ : List MVarId) (t : Expr) (p : Expr) : MetaM (List MVarId ×
       - rewrite on f happened
       - rewrite on e happened
     -/
-    let Tf ← inferType <| ← whnf f
+    let Tf ← whnf <| ← inferType f
     let (_τ, σ) ← match Tf.arrow? with
     | .some (τ, σ) => pure (τ, σ)
-    | .none => throwError "Type of f in f e must be of the form σ → τ"
+    | .none => throwError "Type of f in f e must be of the form σ → τ but is {Tf}"
     -- precondition: type(Γ, Ψ, f)↑ ≡ τ → σ
     let rel ← mkFreshExprMVar <| mkRel σ
-    let sub ← mkFreshExprMVar <| mkApp2 (mkConst ``Subrel) F <| mkApp2 (mkConst ``respectful) E rel
-    pure (Ψ ∪ [sub.mvarId!, rel.mvarId!], sub, .app f e, p)
+    let sub ← mkFreshExprMVar <| mkApp2 (mkConst ``Subrel [0]) F <| mkApp2 (mkConst ``respectful [0, 0]) E rel
+    -- TODO is Subrel.subrelation correct here?
+    let p := mkApp7 (mkConst ``Subrel.subrelation [0]) sub f f' pf e e' pe
+    pure (Ψ ∪ [sub.mvarId!, rel.mvarId!], sub, .app f' e', p)
   | .lam n T b i => do
-    logInfo m!"Lam {t}"
+    trace[Meta.Tactic.grewrite] "LAM {t}"
     let (Ψ, S, b, p) ← rew Ψ b p
     /-
     preconditions:
@@ -128,11 +162,10 @@ partial def rew (Ψ : List MVarId) (t : Expr) (p : Expr) : MetaM (List MVarId ×
     let S := mkApp2 (mkConst ``pointwiseRelation) T S
     pure (Ψ, S, .lam n T b i, p)
   | .forallE n T b i => do
-    logInfo m!"Pi {t}"
-    let (Ψ', p', u, unifyable) ← unifyStar Ψ T p
+    trace[Meta.Tactic.grewrite] "PI {t}"
+    let (Ψ', r, p', u, unifyable) ← unifyStar Ψ T p
     if unifyable then
-      let (R, _, _) ← isRelation p
-      pure (Ψ', R, u, p')
+      pure (Ψ', r, u, p')
     else
       let (Ψ, S, b, p) ← rew Ψ (mkApp (mkConst ``all) <| .lam n T b i) p
       /-
@@ -146,21 +179,33 @@ partial def rew (Ψ : List MVarId) (t : Expr) (p : Expr) : MetaM (List MVarId ×
         throwError "Rewrite of `all λ x ↦ y` resulted in a different (thus wrong) type."
   | _ => match t.arrow? with
   | .some (α, β) =>
-    logInfo m!"Arrow {t}"
-    let (Ψ, S, b, p) ← rew Ψ (mkApp2 (mkConst ``Impl) α β) p
+    trace[Meta.Tactic.grewrite] "Arrow {t}"
+    let (Ψ, S, b, p) ← rew Ψ (mkApp2 (mkConst ``impl) α β) p
     if let .app (.app _c α) β := b then
       pure (Ψ, S, ← mkArrow α β, p)
     else
       throwError "Rewrite of `Impl α β` resulted in a different (thus wrong) type."
   | .none => do
-    logInfo m!"Atom {t}"
+    trace[Meta.Tactic.grewrite] "ATOM {t}"
     atom Ψ t p
 
-def proofSearch (constraints : List MVarId) (p : Expr) : MetaM Unit := do
-  sorry
+  -- iterate over constraits and call synthInstance
+def proofSearchGoal (Ψ : List MVarId) (R : Expr) (u : Expr) (p : Expr) : TacticM Unit := do
+  let R := mkApp (mkConst ``Subrel [0]) <| mkApp R (← mkAppM ``flip #[mkConst ``impl])
+  let sub ← mkFreshExprMVar R
+  let p ← mkAppOptM ``Subrel.subrelation #[none, none, none, sub, none, none, p]
+  let Ψ := Ψ.insert sub.mvarId!
+
+  -- Try to solve the constraints with `typeclasses_eauto with grewrite`
+  let success ← Eauto.eautoMain Ψ #[`grewrite] true
+  if !success then
+    throwError "grewrite: unable to solve constraints"
+  let goal ← getMainGoal
+  let subgoals ← goal.apply (← instantiateMVars p)
+  replaceMainGoal subgoals
 
 def algorithm (ps : Syntax.TSepArray `ident ",") : TacticM Unit := withMainContext do
-  let p ← getMainGoal
+  withTraceNode `Meta.Tactic.grewrite (fun _ => return m!"algorithm") do
   let lctx ← getLCtx
   -- Confirm all passed lemmas are in the local context
   let mut ldecls : List LocalDecl := []
@@ -172,18 +217,58 @@ def algorithm (ps : Syntax.TSepArray `ident ",") : TacticM Unit := withMainConte
       else
         continue
   for ldecl in ldecls do
-    let t := ldecl.type
-    let p := mkMVar p
-    let p := ← inferType p
+    let goal ← getMainGoal
+    let p ← inferType ldecl.toExpr
+    let t ← goal.getType
     let Ψ := []
-    let (Ψ, _R, _u, _p) ← rew Ψ p t
-    logInfo m!"{Ψ}"
+    let (Ψ, R, u, p) ← rew Ψ t p
+    trace[Meta.Tactic.grewrite] "{Ψ}"
+    proofSearchGoal Ψ R u p
 
-elab "myrw" "[" ps:ident,+ "]" : tactic =>
+elab "grewrite" "[" ps:ident,+ "]" : tactic =>
   algorithm ps
 
-example : ∀ {α : Type} {r : α → α → Prop} {x y z : α}, [Transitive r] → r x y → r y z → r x z := by
+end Tactic
+
+set_option trace.Meta.Tactic.grewrite true
+
+example : ∀ {α : Sort u} {r : relation α} {x y z : α}, [Transitive r] → r x y → r y z → r x z := by
   intro a r x y z t h h₀
-  myrw [h]
-  --assumption
+  grewrite [h]
   sorry
+
+variable (α β γ: Type)
+variable (Rα: relation α) (Rβ: relation β) (Rγ: relation γ)
+variable (Pα: α → Prop) (Pβ: β → Prop) (Pγ: γ → Prop)
+variable (Pαβγ: α → β → Prop)
+variable (fαβ: α → β) (fβγ: β → γ)
+variable [Proper_fαβ: Proper (Rα ⟹ Rβ) fαβ]
+variable [Proper_Pα: Proper (Rα ⟹ Iff) Pα]
+
+example (h: Rα a a') (finish: Pα a') : Pα a := by
+  grewrite [h]
+  exact finish
+
+example (h: Rα a a') : Rα a x := by
+  grewrite [h]
+  sorry
+
+example (h: Rα a a') (finish: Pα a') : Pα a := by
+  grewrite [h]
+  assumption
+
+-- Rewrite a PER within itself
+example (h: Rα a a') (finish: Rα a' x) : Rα a x := by
+  grewrite [h]
+  assumption
+example (h: Rα a a') (finish: Rα x a') : Rα x a := by
+  grewrite [h]
+  assumption
+
+example (h: Rα a a') (finish: Rβ (fαβ a') x): Rβ (fαβ a) x := by
+  grewrite [h]
+  assumption
+
+example (h: Rα a a') (finish: Rα a' a'): Rα a a := by
+  grewrite [h]
+  assumption
