Grw/Test.lean
@@ -1,0 +1,41 @@
+import Grw.Tactic
+import Grw.Morphism
+
+open Morphism
+
+-- Examples
+set_option trace.Meta.Tactic.grewrite true
+
+example : ∀ {α : Type} {r : α → α → Prop} {x y z : α}, [Transitive r] → r x y → r y z → r x z := by
+  intro a r x y z t h h₀
+  grewrite [h]
+
+  assumption
+
+variable (α β γ: Type)
+variable (Rα: relation α) (Rβ: relation β) (Rγ: relation γ)
+variable (Pα: α → Prop) (Pβ: β → Prop) (Pγ: γ → Prop)
+variable (Pαβγ: α → β → Prop)
+variable (fαβ: α → β) (fβγ: β → γ)
+variable [Proper_fαβ: Proper (Rα ⟹ Rβ) fαβ]
+variable [Proper_Pα: Proper (Rα ⟹ Iff) Pα]
+
+example (h: Rα a a') (finish: Pα a') : Pα a := by
+  grewrite [h]
+  assumption
+
+-- Rewrite a PER within itself
+example (h: Rα a a') (finish: Rα a' x) : Rα a x := by
+  grewrite [h]
+  assumption
+example (h: Rα a a') (finish: Rα x a') : Rα x a := by
+  grewrite [h]
+  assumption
+
+example (h: Rα a a') (finish: Rβ (fαβ a') x): Rβ (fαβ a) x := by
+  grewrite [h]
+  assumption
+
+example (h: Rα a a') (finish: Rα a' a'): Rα a a := by
+  grewrite [h]
+  assumption
