README.md
@@ -1,1 +1,8 @@
 # grw
+
+## Questions
+
++ Quick note: equivalence relations are not closed under the respectful morphism construction so we actually have to start at PERs. It's mostly the same, fortunately.
++ Reading the Coq source code, it also turns out that a fair amount of typeclass resolution is customized by using the fact that the typeclass resolution engine is a variant of eauto
++ By using hints that call into custom tactics, a number of instances are applied selectively and not put into the instance database, to avoid combinatorial explosions.
++ Unlike the standard synthesis algorithm, this will instantiate metavariables.
